src/spec/core/TLS13.Wire.Spec.fst
@@ -1122,6 +1122,8 @@ let lemma_parse_tls_message_round_trip
         Seq.equal fragment (serialize_handshake (M.Certificate c))
       | Some (M.TlsHandshake (M.CertificateVerify cv)) ->
         Seq.equal fragment (serialize_handshake (M.CertificateVerify cv))
+      | Some (M.TlsHandshake (M.Finished fin)) ->
+        Seq.equal fragment (serialize_handshake (M.Finished fin))
       | _ -> True))
 =
   match content_type with
